SortedList/Imperative.lean
@@ -25,24 +25,81 @@ def unique (xs : List Int) : List Int := Id.run do
 
 #eval unique [1, 1, 2, 2, 3]
 
-/-- Every element in the input is in the output -/
+/-- The key properties that a `unique` function must have together defines its specification. -/
+structure UniqueSpec (unique : List Int → List Int) where
+  /-- Every element in the input is in the output -/
+  supset : ∀ l, l ⊆ unique l
+  /-- Every element in the output is in the input -/
+  subset : ∀ l, unique l ⊆ l
+  /-- The output is sorted if the input is sorted -/
+  sorted_if_sorted : ∀ l, (Sorted l) → Sorted (unique l)
+  /-- The output contains no duplicates if the input is sorted -/
+  nodup_if_sorted : ∀ l, (Sorted l) → Nodup (unique l)
+
+
 theorem unique_spec_supset (l : List Int) : l ⊆ unique l := by
+  generalize h : unique l = r
+  apply Id.by_wp h _
+  -- simp only [wp, Id.run, PredTrans.pure_apply]
+
+  -- Using the monadic verification condition generator, we can split the proof into 4 steps.
+  mvcgen
+
+  -- First, we need to provide an invariant that holds before, during, and after the for loop.
+  case inv =>
+    exact ⇓⟨⟨c, out⟩, xs⟩ =>
+        (∀ x, some x = c → x ∈ out) ∧ -- First invariant: c is always in out
+        xs.pref ⊆ out -- Second invariant: main property (`l ⊆ unique l`) holds for out
+
+  -- We can simplify all goals to see the individual steps better
+  -- clear c out
+  -- obtain ⟨c, out⟩ := b
+  all_goals dsimp at *
+  all_goals simp only [reverse_subset, true_imp_iff] at *
+
+  -- The first two goals state that assuming that the invariant holds before the loop iteration (`h`), the invariant holds after the loop iteration.
+  -- There are two goals to analyze both code branches of `if some x != c then ...`
+  -- The next goal `pre1` states that the invariant holds before the loop.
+
+  -- Proof automation (the simplifier) takes care of the first three goals.
+  all_goals simp_all
+
+  -- The last goal states that if the loop condition holds after the loop, the main statement `l ⊆ unique l` holds.
+  case post.success =>
+    clear c out
+    expose_names
+    obtain ⟨c, out⟩ := r_1
+    dsimp
+    intro inv1 inv2
+    simp only [wp, Id.run, PredTrans.pure_apply]
+    exact inv2
+
+theorem unique_spec_subset (l : List Int) : unique l ⊆ l := by
   generalize h : unique l = r
   apply Id.by_wp h _
   mvcgen
   case inv =>
     exact ⇓⟨⟨c, out⟩, xs⟩ =>
         (∀ x, some x = c → x ∈ out) ∧ -- c is always in out
-        xs.pref ⊆ out -- property holds for out
+        out ⊆ xs.pref -- property holds for out
 
   all_goals simp_all
+  case pre1 =>
+    rfl
   case post.success =>
-    intros
-    assumption
+    intro h1 h2
+    exact h2
 
+-- A list is strictly sorted if every element is strictly less than the next
 abbrev StrictSorted (xs : List Int) := Pairwise (· < ·) xs
 
-/-- Main lemma: Given a sorted list as input, `unique` returns a strictly sorted list. -/
+theorem StrictSorted.sorted (h : StrictSorted xs) : Sorted xs := by grind
+
+theorem StrictSorted.nodup (h : StrictSorted xs) : Nodup xs := by grind
+
+theorem StrictSorted.iff : StrictSorted xs ↔ Sorted xs ∧ Nodup xs := by grind
+
+/-- Key lemma: Given a sorted list as input, `unique` returns a strictly sorted list. -/
 theorem unique_spec_strictSorted (l : List Int) (hl : Sorted l) : StrictSorted (unique l) := by
   generalize h : unique l = r
   apply Id.by_wp h _
@@ -74,20 +131,19 @@ theorem unique_spec_strictSorted (l : List Int) (hl : Sorted l) : StrictSorted (
     grind
   · grind
 
-theorem StrictSorted.sorted (h : StrictSorted xs) : Sorted xs := by grind
-
--- Adversarially defining `unique` to be the identity function already satisfies the superset property and order preservation, however the correct implementation returns a strictly increasing list, which means there are no duplicate elements.
-theorem StrictSorted.nodup (h : StrictSorted xs) : Nodup xs := by grind
-
-theorem StrictSorted.iff : StrictSorted xs ↔ Sorted xs ∧ Nodup xs := by grind
-
 /-- An example for composing above results -/
-theorem unique_spec_nodup (l : List Int) (hl : Sorted l) : Nodup (unique l) := by
+theorem unique_nodup (l : List Int) (hl : Sorted l) : Nodup (unique l) := by
   apply StrictSorted.nodup
   exact unique_spec_strictSorted l hl
 
-/-- The key property that `unique` must have: Every element in the input is in the output and the output is strictly increasing (or equivalently, doesn't contain duplicates and is sorted). -/
-theorem unique_spec (l : List Int) (hl : Sorted l) : let r := unique l; l ⊆ r ∧ StrictSorted r := by
-  constructor
+/-- Main statement: `unique` satisfies the specification. -/
+theorem unique_spec : UniqueSpec unique := by
+  constructor <;> intro l
   · exact unique_spec_supset l
-  · exact unique_spec_strictSorted l hl
+  · exact unique_spec_subset l
+  · intro hl
+    apply StrictSorted.sorted
+    exact unique_spec_strictSorted l hl
+  · intro hl
+    apply StrictSorted.nodup
+    exact unique_spec_strictSorted l hl
